\documentclass[12pt, a4paper]{article}

\usepackage{amsmath}
\usepackage{amssymb}
\usepackage{amsthm}
\usepackage[a4paper, portrait, margin=1in]{geometry}

\newcommand{\R}{\mathbb{R}}
\newcommand{\Z}{\mathbb{Z}}
\newcommand{\N}{\mathbb{N}}
\renewcommand{\qedsymbol}{$\blacksquare$}

\newcommand{\sse}{\subseteq}

\newcommand{\emptyline}{\hfill\break}

\newtheorem{theorem}{Theorem}

% let's begin
\begin{document}

\noindent\textbf{(Q2)}

\vspace{5mm}

\noindent\textit{(a)} $\displaystyle{\frac{1}{36}}$

\vspace{5mm}

\noindent\textit{(b)} $\displaystyle{\frac{1}{(n + 1)^2}}$

\vspace{5mm}

\noindent\textit{(c)}

\begin{proof}
    Let the theorem $P(k)$ be $\prod_{i = 1}^k\frac{i^2}{(i + 1)^2} = \frac{1}{(k + 1)^2}$.
    
    We prove this theorem by considering the base case $P(1)$ and then the induction hypothesis
    $P(k) \implies P(k + 1)$ for some $k \in \N$:
    \[
        \prod_{i = 1}^k\frac{i^2}{(i + 1)^2}
        = \frac{1}{(k + 1)^2}
        \implies
        \prod_{i = 1}^{k + 1}\frac{i^2}{(i + 1)^2}
        = \frac{1}{((k + 1) + 1)^2}
    \]

    \noindent\textit{Base Case.}
    \[
        P(1) = \prod_{i = 1}^{1}\frac{i^2}{(i + 1)^2} = \frac{1}{4} = \frac{1}{(1 + 1)^2}
    \]

    Which shows the base case holds.

    \noindent\textit{Induction Step.}

    Assuming $P(k)$, it follows:

    \begin{align*}
        \prod_{i = 1}^{k + 1}  & = \frac{1}{(k + 1)^2} \cdot \frac{(k + 1)^2}{((k + 1) + 1)^2}\\
        & = \frac{(k + 1)^2}{(k + 1)^2((k + 1) + 1)^2}\\
        & = \frac{1}{((k + 1) + 1)^2}
    \end{align*}

    By PMI, since both the base case and induction step hold, we have proven the theorem, as required.

\end{proof}

\end{document}