\documentclass[12pt, a4paper]{article}

\usepackage{amsmath}
\usepackage{amssymb}
\usepackage{amsthm}
\usepackage[a4paper, portrait, margin=1in]{geometry}

\newcommand{\R}{\mathbb{R}}
\newcommand{\Z}{\mathbb{Z}}
\newcommand{\N}{\mathbb{N}}
\renewcommand{\qedsymbol}{$\blacksquare$}

\newcommand{\emptyline}{\hfill\break}

\newtheorem{theorem}{Theorem}

% let's begin
\begin{document}

\noindent\textbf{(Q3)}

\vspace{5mm}

\noindent\textit{(a)} $\displaystyle{\frac{5}{6}}$\

\vspace{5mm}

\noindent\textit{(b)} $\displaystyle{\frac{n}{n + 1}}$

\vspace{5mm}

\noindent\textit{(c)}

\begin{proof}
    Let the theorem be $P(k)$ be $\sum_{i =  1}^{k}(\frac{1}{i} - \frac{1}{i + 1}) = \frac{k}{k + 1}$.
    
    We prove this by considering the base case $P(1)$ and then the induction hypothesis
    $P(k) \implies P(k + 1)$ for some $k \in \N$:
    \[
        \sum_{i = 1}^{k}\left(\frac{1}{i} - \frac{1}{i + 1}\right) = \frac{k}{k + 1}
        \implies
        \sum_{i = 1}^{k + 1}\left(\frac{1}{i} - \frac{1}{i + 1}\right) = \frac{k + 1}{(k + 1) + 1}
    \]

    \noindent\textit{Base Case.}
    \[
        P(1) = \sum_{i = 1}^{1}\left(\frac{1}{1} - \frac{1}{1 + 1}\right)
        = \frac{1}{2} = \frac{1}{1 + 1}
    \]

    \noindent\textit{Induction Step.}

    Assuming $P(k)$, it follows:
    \begin{align*}
        \sum_{i = 1}^{k + 1}\left(\frac{1}{i} - \frac{1}{i + 1}\right) & =
        \frac{k}{k + 1} + \left(\frac{1}{k + 1} - \frac{1}{(k + 1) + 1}\right)\\
        & = \frac{k}{k + 1} + \left(\frac{(k + 1) + 1}{(k + 1)((k + 1) + 1)} - 
        \frac{k + 1}{(k + 1)((k + 1) + 1)}\right)\\
        & = \frac{k}{k + 1} + \left(\frac{1}{(k + 1)((k + 1) + 1)}\right)\\
        & = \frac{k((k + 1) + 1) + 1}{(k + 1)((k + 1) + 1)}\\
        & = \frac{k^2 + 2k + 1}{(k + 1)((k + 1) + 1)}\\
        & = \frac{(k + 1)^2}{(k + 1)((k + 1) + 1)}\\
        & = \frac{k + 1}{(k + 1) + 1}
    \end{align*}

    Which proves the induction hypothesis.

    Since the base case and induction hypothesis both hold, the theorem is proved
    by induction, as required.

\end{proof}

\end{document}