\documentclass[12pt, a4paper]{article}

\usepackage{amsmath}
\usepackage{amssymb}
\usepackage{amsthm}
\usepackage[a4paper, portrait, margin=1in]{geometry}

\newcommand{\R}{\mathbb{R}}
\newcommand{\Z}{\mathbb{Z}}
\newcommand{\N}{\mathbb{N}}
\renewcommand{\qedsymbol}{$\blacksquare$}

\newcommand{\emptyline}{\hfill\break}

\newtheorem{theorem}{Theorem}

% let's begin
\begin{document}

\noindent\textbf{(Q4)}

\begin{theorem}
    Let $x \in (0, 1)$. Use induction to prove that $\frac{1}{x^n} > \frac{1}{x}$ for all
    natural numbers $n \geq 2$.
\end{theorem}

\begin{proof}
    Let the theorem be $P(n)$ such that:
    \begin{gather*}
        \forall x \in (0,1), \forall n \in \N \text{ where $n \geq 2$},\\
        \frac{1}{x^n} > \frac{1}{x}
    \end{gather*}
    We observe the following:
    \begin{gather}
        \frac{1}{x^n} > \frac{1}{x} \iff x^n < x
    \end{gather}

    It thus suffices to prove that $x^n < x$.

    Using induction we consider a base case $P(2)$ and the induction hypothesis
    $P(k) \implies P(k + 1)$.

    \noindent\textit{Base Case.}
    
    \[
        P(2) = \frac{1}{x^2} > \frac{1}{x}
    \]

    Since $0 < x < 1$:
    \[
        x < 1 \implies x^2 < x \iff \frac{1}{x^2} > \frac{1}{x}
    \]

    Thus, the base case holds.

    \noindent\textit{Induction Step.}

    We consider the induction hypothesis $P(k) \implies P(k + 1)$:
    \[
        \frac{1}{x^k} > \frac{1}{x} \implies \frac{1}{x^{k + 1}} > \frac{1}{x}
    \]

    By (1), we can rewrite this as $x^k < x \implies x^{k + 1} < x$.

    We observe that $x^{k + 1} = x^k \cdot x$. Assuming $P(k)$, it follows:
    \begin{align*}
        x^k < x & \implies x^k \cdot x < x \text{ (since $x < 1$)}\\
        & \implies x^{k + 1} < x \iff \frac{1}{x^{k + 1}} > \frac{1}{x}
    \end{align*}

    By PMI, since the base case and induction hypothesis both hold, the theorem is proved,
    as required.

\end{proof}

\end{document}